Update squeeze function in Spec.SHA3.Vec

code/sha3/Hacl.Spec.SHA3.Vec.fst
@@ -483,34 +483,162 @@ let absorb
   let s = absorb_last #a #m delimitedSuffix rateInBytes rem mb s in
   s
 
+noextract
+let init_b1 (#m:m_spec{lanes m == 1})
+            (outputByteLen:size_nat) :
+            multiseq (lanes m) outputByteLen =
+  let l = create outputByteLen (u8 0) in
+  ntup1 l
+
+noextract
+let init_b4 (#m:m_spec{lanes m == 4})
+            (outputByteLen:size_nat) :
+            multiseq (lanes m) outputByteLen =
+  let l0 = create outputByteLen (u8 0) in
+  let l1 = create outputByteLen (u8 0) in
+  let l2 = create outputByteLen (u8 0) in
+  let l3 = create outputByteLen (u8 0) in
+  ntup4 (l0, (l1, (l2, l3)))
+
+noextract
+let init_b (#m:m_spec{is_supported m})
+           (outputByteLen:size_nat) :
+           multiseq (lanes m) outputByteLen =
+  match lanes m with
+  | 1 -> init_b1 #m outputByteLen
+  | 4 -> init_b4 #m outputByteLen
+
+#push-options "--z3rlimit 200"
+noextract
+let update_b1 (#m:m_spec{lanes m == 1})
+              (block:lseq uint8 (lanes m * 256))
+              (rateInBytes:size_nat{0 < rateInBytes /\ rateInBytes <= 256})
+              (outputByteLen:size_nat)
+              (i:size_nat{i < outputByteLen / rateInBytes})
+              (b:multiseq (lanes m) outputByteLen):
+              multiseq (lanes m) outputByteLen =
+  let l = tup1 b in
+  let l = update_sub #uint8 #outputByteLen 
+    l (i * rateInBytes) rateInBytes (sub block 0 rateInBytes) in
+  ntup1 l
+#pop-options
+
+#push-options "--z3rlimit 200"
+noextract
+let update_b4 (#m:m_spec{lanes m == 4})
+              (block:lseq uint8 (lanes m * 256))
+              (rateInBytes:size_nat{0 < rateInBytes /\ rateInBytes <= 256})
+              (outputByteLen:size_nat)
+              (i:size_nat{i < outputByteLen / rateInBytes})
+              (b:multiseq (lanes m) outputByteLen):
+              multiseq (lanes m) outputByteLen =
+  let (l0, (l1, (l2, l3))) = tup4 b in
+  let l0 = update_sub #uint8 #outputByteLen
+    l0 (i * rateInBytes) rateInBytes (sub block 0 rateInBytes) in
+  let l1 = update_sub #uint8 #outputByteLen
+    l1 (i * rateInBytes) rateInBytes (sub block 256 rateInBytes) in
+  let l2 = update_sub #uint8 #outputByteLen
+    l2 (i * rateInBytes) rateInBytes (sub block 512 rateInBytes) in
+  let l3 = update_sub #uint8 #outputByteLen
+    l3 (i * rateInBytes) rateInBytes (sub block 768 rateInBytes) in
+  ntup4 (l0, (l1, (l2, l3)))
+#pop-options
+
+noextract
+let update_b (#m:m_spec{is_supported m})
+             (block:lseq uint8 (lanes m * 256))
+             (rateInBytes:size_nat{0 < rateInBytes /\ rateInBytes <= 256})
+             (outputByteLen:size_nat)
+             (i:size_nat{i < outputByteLen / rateInBytes})
+             (b:multiseq (lanes m) outputByteLen):
+             multiseq (lanes m) outputByteLen =
+  match lanes m with
+  | 1 -> update_b1 #m block rateInBytes outputByteLen i b
+  | 4 -> update_b4 #m block rateInBytes outputByteLen i b
+
+#push-options "--z3rlimit 200"
+noextract
+let update_b_last1 (#m:m_spec{lanes m == 1})
+              (block:lseq uint8 (lanes m * 256))
+              (rateInBytes:size_nat{0 < rateInBytes /\ rateInBytes <= 256})
+              (outputByteLen:size_nat)
+              (outRem:size_nat{outRem == outputByteLen % rateInBytes})
+              (b:multiseq (lanes m) outputByteLen):
+              multiseq (lanes m) outputByteLen =
+  FStar.Math.Lemmas.lemma_mod_lt outputByteLen rateInBytes;
+  let l = tup1 b in
+  let l = update_sub #uint8 #outputByteLen 
+    l (outputByteLen / rateInBytes) outRem (sub block 0 outRem) in
+  ntup1 l
+#pop-options
+
+#push-options "--z3rlimit 200"
+noextract
+let update_b_last4 (#m:m_spec{lanes m == 4})
+              (block:lseq uint8 (lanes m * 256))
+              (rateInBytes:size_nat{0 < rateInBytes /\ rateInBytes <= 256})
+              (outputByteLen:size_nat)
+              (outRem:size_nat{outRem == outputByteLen % rateInBytes})
+              (b:multiseq (lanes m) outputByteLen):
+              multiseq (lanes m) outputByteLen =
+  FStar.Math.Lemmas.lemma_mod_lt outputByteLen rateInBytes;
+  let (l0, (l1, (l2, l3))) = tup4 b in
+  let l0 = update_sub #uint8 #outputByteLen
+    l0 (outputByteLen / rateInBytes) outRem (sub block 0 outRem) in
+  let l1 = update_sub #uint8 #outputByteLen
+    l1 (outputByteLen / rateInBytes) outRem (sub block 256 outRem) in
+  let l2 = update_sub #uint8 #outputByteLen
+    l2 (outputByteLen / rateInBytes) outRem (sub block 512 outRem) in
+  let l3 = update_sub #uint8 #outputByteLen
+    l3 (outputByteLen / rateInBytes) outRem (sub block 768 outRem) in
+  ntup4 (l0, (l1, (l2, l3)))
+#pop-options
+
+noextract
+let update_b_last (#m:m_spec{is_supported m})
+             (block:lseq uint8 (lanes m * 256))
+             (rateInBytes:size_nat{0 < rateInBytes /\ rateInBytes <= 256})
+             (outputByteLen:size_nat)
+             (outRem:size_nat{outRem == outputByteLen % rateInBytes})
+             (b:multiseq (lanes m) outputByteLen):
+             multiseq (lanes m) outputByteLen =
+  match lanes m with
+  | 1 -> update_b_last1 #m block rateInBytes outputByteLen outRem b
+  | 4 -> update_b_last4 #m block rateInBytes outputByteLen outRem b
+
 let squeeze_inner
   (#a:keccak_alg)
   (#m:m_spec{is_supported m})
   (rateInBytes:size_nat{0 < rateInBytes /\ rateInBytes <= 256})
   (outputByteLen:size_nat)
-  (i:size_nat{i < outputByteLen / (lanes m * 256)})
-  (s:state m) :
-  Tot ((state m) & lseq uint8 (lanes m * 32 * word_length a)) =
+  (i:size_nat{i < outputByteLen / rateInBytes})
+  (s, b) :
+  ((state m) & (multiseq (lanes m) outputByteLen)) =
 
   let block = storeState #a #m s in
+  let b = update_b #m block rateInBytes outputByteLen i b in
   let s = state_permute m s in
-  s, block
+  s, b
+
+val squeeze_s: 
+  m:m_spec -> rateInBytes:size_nat{0 < rateInBytes /\ rateInBytes <= 256} ->
+  outputByteLen:size_nat -> i:size_nat{i <= outputByteLen / rateInBytes} -> Type0
+let squeeze_s m rateInBytes outputByteLen i = (state m) & (multiseq (lanes m) outputByteLen)
 
 let squeeze
   (#a:keccak_alg)
   (#m:m_spec{is_supported m})
   (s:state m)
   (rateInBytes:size_nat{0 < rateInBytes /\ rateInBytes <= 256})
-  (outputByteLen:size_nat{outputByteLen % (lanes m * 256) == 0}):
-  Tot (lbytes outputByteLen) =
-
-  let outBlocks = outputByteLen / (lanes m * 256) in
-  let sm (i:nat{i <= outBlocks}) = state m in
-  let s, output =
-    generate_blocks (lanes m * 32 * word_length a) outBlocks outBlocks sm
-      (squeeze_inner #a #m rateInBytes outputByteLen) s
-  in
-  to_lseq output
+  (outputByteLen:size_nat) :
+  Tot (multiseq (lanes m) outputByteLen) =
+  let b = init_b #m outputByteLen in
+  let outBlocks = outputByteLen / rateInBytes in
+  let s, b = repeat_gen outBlocks (squeeze_s m rateInBytes outputByteLen)
+    (squeeze_inner #a #m rateInBytes outputByteLen) (s, b) in
+  let remOut = outputByteLen % rateInBytes in
+  let block = storeState #a #m s in
+  update_b_last #m block rateInBytes outputByteLen remOut b
 
 val keccak:
     #a:keccak_alg
@@ -519,8 +647,8 @@ val keccak:
   -> inputByteLen:nat
   -> input:multiseq (lanes m) inputByteLen
   -> delimitedSuffix:byte_t
-  -> outputByteLen:size_nat{outputByteLen % (lanes m * 256) == 0} ->
-  Tot (lbytes outputByteLen)
+  -> outputByteLen:size_nat ->
+  Tot (multiseq (lanes m) outputByteLen)
 
 let keccak #a #m rate inputByteLen input delimitedSuffix outputByteLen =
   let rateInBytes = rate / 8 in
